rocq/theories/TypeSystem/TypeChecker.v
@@ -32,6 +32,8 @@ Extraction "../fixtures/TypeChecker.ml"
   infer_core_env_roots_shadow_safe_checked_assoc
   infer_env_roots_shadow_safe_checked_assoc infer_full_env_roots_checked_assoc
   check_fn_root_shadow_summary check_env_root_shadow_summary
+  check_fn_root_shadow_captured_call_store_safe_summary_absent
+  check_env_root_shadow_captured_call_store_safe_summary_absent
   check_fn_root_shadow_provenance_summary
   check_env_root_shadow_provenance_summary
   direct_call_ready_expr_b
